{
 "cells": [
  {
   "cell_type": "markdown",
   "metadata": {},
   "source": [
    "# Sums\n",
    "\n",
    "## Notion Collection\n",
    "$$\n",
    "\\pi(N) := \\text{the number of primes that less equal than N}\n",
    "$$\n",
    "\n",
    "$$\n",
    "\\pi(N) \\approx \\ln\\ln N + M \\\\\n",
    "M \\approx 0.261~497~212~847~642~783~755~426~838~608~695~859~051~566~6\n",
    "$$\n",
    "\n",
    "We can put proposition into $[~~]$:\n",
    "$$\n",
    "[p] = \\begin{cases}\n",
    "    1, p \\\\\n",
    "    0, \\neg p\n",
    "\\end{cases}\n",
    "$$\n",
    "\n",
    "## Sums and Recurrences\n",
    "We can use the same method in sums:\n",
    "$$\n",
    "S_0 = \\alpha \\\\\n",
    "S_n = S_{n - 1} + \\beta + \\gamma n\n",
    "$$\n",
    "Write it in the form:\n",
    "$$\n",
    "S_n  = A(n)\\alpha + B(n)\\beta + C(n)\\gamma\n",
    "$$\n",
    "Simply let $R_n = 1, n, n^2$ (more items for higher degree),\n",
    "$$\n",
    "A(n) = 1\\\\\n",
    "B(n) = n,\n",
    "C(n) = \\frac{n(n + 1)}{2}\n",
    "$$\n",
    "Thus, for any sum in the form of $\\sum_{i = 0}^n(a + bi)$, the close form will be:\n",
    "$$\n",
    "a(n + 1) + b\\frac{n(n + 1)}{2}\n",
    "$$\n",
    "\n",
    "On the other hand, any recursion formula in the following form can be transformed into summation:\n",
    "$$\n",
    "a_n T_n = b_nT_{n - 1} +c_n\n",
    "$$\n",
    "Find a $s_n$, s.t.\n",
    "$$\n",
    "s_nb_n = s_{n - 1}a_{n - 1}\n",
    "$$\n",
    "Multiply $s_n$ on both side \n",
    "$$\n",
    "s_n a_n T_n = s_nb_nT_{n - 1} +s_nc_n\n",
    "$$\n",
    "Let $S_n = s_na_nT_n$, then we get\n",
    "$$\n",
    "S_n = S_{n - 1} + s_nc_n\n",
    "$$\n",
    "Therefore,\n",
    "$$\n",
    "S_n = s_0a_0T_0 + \\sum_{k = 1}^ns_kc_k = s_1b_1T_0 + \\sum_{k = 1}^ns_kc_k\n",
    "$$\n",
    "The solution should be\n",
    "$$\n",
    "T_n = \\frac{{s_1b_1T_0 + \\sum_{k = 1}^ns_kc_k}}{s_na_n} \n",
    "$$\n",
    "In fact, $s_n$ can be calculated by,\n",
    "$$\n",
    "s_n = C \\times \\frac{\\prod_{1}^{n - 1}a_i}{\\prod_{2}^{n}b_j}\n",
    "$$\n",
    "For example, for hanoi problem, $a_n = 1$, $b_n = 2$, then we can choose $s_n = 2^{-n}$\n",
    "\n",
    "\n",
    "## Solve the Formula of Quick Sort\n",
    "$$\n",
    "C_0 = C_1 = 0\\\\\n",
    "C_n = n + 1 + \\frac{2}{n} \\sum_{k = 1}^{n - 1}C_k, n \\gt 1\n",
    "$$\n",
    "Solution:\n",
    "\n",
    "multiply $n$ on both side:\n",
    "$$\n",
    "nC_n = n^2 + n + 2 \\sum_{k = 1}^{n - 1}C_k \n",
    "$$\n",
    "substitute $n$ with $(n - 1)$:\n",
    "$$\n",
    "(n - 1)C_{n - 1} = (n - 1)^2 + (n - 1) + 2 \\sum_{k = 1}^{n - 2}C_k\n",
    "$$\n",
    "do subtraction of the two equations we have got:\n",
    "$$\n",
    "nC_n - (n - 1)C_{n - 1} = 2n + 2C_{n - 1}\n",
    "$$\n",
    "by simplification,\n",
    "$$\n",
    "C_0 = C_1 = 0\\\\\n",
    "C_2 = 3\\\\\n",
    "nC_n = (n + 1)C_{n - 1} + 2n\n",
    "$$\n",
    "Let $a_n = n, b_n = n + 1, c_n = 2n - 2[n = 1] + 2[n = 2]$, we can choose $s_n$ as\n",
    "$$\n",
    "s_n = \\frac{2}{n(n + 1)}\n",
    "$$\n",
    "Then, the solution should be\n",
    "$$\n",
    "C_n = 2(n + 1)\\sum_{k = 1}^n\\frac{1}{k + 1} - \\frac{2}{3}(n + 1)\n",
    "$$\n",
    "transform to harmonic numbers:\n",
    "$$\n",
    "\\sum_{k = 1}^{n}\\frac{1}{k + 1} = H_n - 1 + \\frac{1}{n + 1} \\\\\n",
    "C_n = 2(n + 1)H_n - \\frac{8}{3}n - \\frac{2}{3}, n \\gt 1\n",
    "$$\n",
    "\n",
    "## Manipulation of sums\n",
    "### properties of summation\n",
    "$$\n",
    "\\sum ca_k = c\\sum a_k \\\\\n",
    "\\sum (a_k + b_k) = \\sum a_k + \\sum b _k \\\\\n",
    "\\sum_{k \\in K} a_k = \\sum_{p(k) \\in K} a_{p(k)}\n",
    "$$\n",
    "\n",
    "#### Example\n",
    "$$\n",
    "\\begin{aligned}\n",
    "S  &= \\sum_{k = 0}^n(a + bk) \\\\\n",
    "S  &= \\sum_{n - k = 0}^n(a + b(n - k)) = \\sum_{k = 0}^n(a + bn - bk) \\\\\n",
    "2S &= \\sum_{n - k = 0}^n(2a + bn)\\\\\n",
    "S  &= (a + \\frac{1}{2}bn)(n + 1) \n",
    "\\end{aligned}\n",
    "$$\n",
    "\n",
    "### Perturbation Method\n",
    "$$\n",
    "S_n + a_{n + 1} = a_0 + \\sum_{0 \\le k \\le n}a_{k + 1}\n",
    "$$\n",
    "\n",
    "#### Example\n",
    "$$\n",
    "S_n = \\sum_{0 \\le k \\le n} ax^k\n",
    "$$\n",
    "by perturbation method,\n",
    "$$\n",
    "\\begin{aligned}\n",
    "S_n + ax^{n + 1} &= a + \\sum_{0 \\le k \\le n}ax^{k + 1} \\\\\n",
    "&= a + x\\sum_{0 \\le k \\le n}ax^k\\\\\n",
    "&= a + xS_n\n",
    "\\end{aligned}\n",
    "$$\n",
    "Then we get the close form.\n",
    "\n",
    "## Multiple Sums\n",
    "### Transformation\n",
    "$$\n",
    "\\sum_{j\\in J}\\sum_{k \\in K}a_{j, k} = \\sum_{k\\in K}\\sum_{j \\in J}a_{j, k} \n",
    "$$\n",
    "and\n",
    "$$\n",
    "\\sum_{j\\in J}\\sum_{k \\in K(j)}a_{j, k} = \\sum_{k\\in K;}\\sum_{j \\in J'(k)}a_{j, k} \\\\\n",
    "\\text{where } [j \\in J][k \\in K(j)] = [k \\in K'][j \\in J'(k)]\n",
    "$$\n",
    "One particular useful transform is\n",
    "$$\n",
    "[1 \\le j \\le n][j \\le k \\le n] = [1 \\le k \\le n][1 \\le j \\le k]\n",
    "$$\n",
    "\n",
    "#### Example 1\n",
    "$$\n",
    "S_{\\vartriangleleft} = \\sum_{1 \\le j \\le k \\le n} a_ja_k\n",
    "$$\n",
    "$$\n",
    "S_{\\vartriangleright} = \\sum_{1 \\le k \\le j \\le n} a_ja_k\n",
    "$$\n",
    "It is trivial that\n",
    "$$\n",
    "S_{\\vartriangleright} = S_{\\vartriangleleft}\n",
    "$$\n",
    "Also, we have\n",
    "$$\n",
    "[1 \\le j \\le k \\le n] + [1 \\le k \\le j \\le n] = [1 \\le j, k \\le n] + [1 \\le j = k \\le n]\n",
    "$$\n",
    "Therefore,\n",
    "$$\n",
    "2S_{\\vartriangleright} = 2S_{\\vartriangleleft} = \\sum_{1 \\le k, j \\le n}a_ja_k + \\sum_{1 \\le k = j \\le n}a_ja_k \n",
    "$$\n",
    "Therefore,\n",
    "$$\n",
    "S_{\\vartriangleleft} = \\frac{1}{2}\\left(\\left(\\sum_{k = 1}^n a_k \\right)^2 + \\sum_{k = 1}^n a_k^2\\right)\n",
    "$$\n",
    "#### Example 2\n",
    "$$\n",
    "S = \\sum_{1 \\le j \\lt k \\le n} (a_k - a_j)(b_k - b_j)\n",
    "$$\n",
    "We have\n",
    "$$\n",
    "[1 \\le j \\lt k \\le n] + [1 \\le k \\lt j \\le n] = [1 \\le j, k \\le n] - [1 \\le j = k \\le n]\n",
    "$$\n",
    "Therefore,\n",
    "$$\n",
    "2S = \\sum_{1 \\le j , k \\le n} (a_k - a_j)(b_k - b_j) - 2\\sum_{1 \\le j = k \\le n} (a_k - a_j)(b_k - b_j) = \\sum_{1 \\le j , k \\le n} (a_k - a_j)(b_k - b_j)\n",
    "$$\n",
    "Expand the result\n",
    "$$\n",
    "\\begin{aligned}\n",
    "&\\sum_{1 \\le j , k \\le n}a_jb_j - \\sum_{1 \\le j , k \\le n}a_jb_k - \\sum_{1 \\le j , k \\le n}a_kb_j + \\sum_{1 \\le j , k \\le n}a_kb_k \\\\\n",
    "=& 2 \\sum_{1 \\le j , k \\le n}a_kb_k - 2\\sum_{1 \\le j , k \\le n}a_jb_k \\\\\n",
    "=& 2n \\sum_{1 \\le k \\le n}a_kb_k - 2\\left(\\sum_{1 \\le k \\le n}a_k\\right)\\left(\\sum_{1 \\le k \\le n }b_k\\right)\n",
    "\\end{aligned}\n",
    "$$\n",
    "We get\n",
    "$$\n",
    "\\left(\\sum_{1 \\le k \\le n}a_k\\right)\\left(\\sum_{1 \\le k \\le n }b_k\\right) = n \\sum_{1 \\le k \\le n}a_kb_k - \\sum_{1 \\le j \\lt k \\le n} (a_k - a_j)(b_k - b_j)\n",
    "$$\n",
    "\n",
    "This is exactly a special form of **Chebyshev's monotonic inequality**:\n",
    "$$\n",
    "\\left(\\sum_{1 \\le k \\le n}a_k\\right)\\left(\\sum_{1 \\le k \\le n }b_k\\right) \\le n \\sum_{1 \\le k \\le n}a_kb_k, a_i \\downarrow \\wedge b_i\\downarrow \\\\\n",
    "\\left(\\sum_{1 \\le k \\le n}a_k\\right)\\left(\\sum_{1 \\le k \\le n }b_k\\right) \\ge n \\sum_{1 \\le k \\le n}a_kb_k, a_i \\downarrow \\wedge b_i\\uparrow\n",
    "$$\n",
    "\n",
    "#### Attempts to Find the Close Form\n",
    "\n",
    "##### Attempts 1\n",
    "$$\n",
    "\\begin{aligned}\n",
    "S_n &= \\sum_{1 \\le k \\le n}\\sum_{1\\le j \\lt k} \\frac{1}{k - j}\\\\\n",
    "    &= \\sum_{1 \\le k \\le n}\\sum_{1\\le k - j \\lt k} \\frac{1}{j}\\\\\n",
    "    &= \\sum_{1 \\le k \\le n}\\sum_{0\\lt j \\le k - 1} \\frac{1}{j}\\\\\n",
    "    &= \\sum_{1 \\le k \\le n} H_{k - 1}\n",
    "\\end{aligned}\n",
    "$$\n",
    "failed\n",
    "##### Attempts 2\n",
    "$$\n",
    "\\begin{aligned}\n",
    "S_n &= \\sum_{1 \\le j \\le n}\\sum_{j\\lt k \\le n} \\frac{1}{k - j}\\\\\n",
    "    &= \\sum_{1 \\le j \\le n}\\sum_{j\\lt k + j \\lt n} \\frac{1}{k}\\\\\n",
    "    &= \\sum_{1 \\le j \\le n}\\sum_{0\\lt k \\le n - j} \\frac{1}{k}\\\\\n",
    "    &= \\sum_{1 \\le j \\le n} H_{n - j}\\\\\n",
    "    &= \\sum_{1 \\le n - j \\le n} H_{j}\\\\\n",
    "    &= \\sum_{0 \\le j \\lt n} H_{j}\\\\\n",
    "\\end{aligned}\n",
    "$$\n",
    "failed\n",
    "##### Attempts 3\n",
    "$$\n",
    "\\begin{aligned}\n",
    "S_n &= \\sum_{1 \\le j\\lt k \\le n} \\frac{1}{k - j}\\\\\n",
    "    &= \\sum_{1 \\le j\\lt k + j \\le n} \\frac{1}{k}\\\\\n",
    "    &= \\sum_{1 \\le k \\le n} \\sum_{1\\lt j \\le n - k} \\frac{1}{k}\\\\\n",
    "    &= \\sum_{1 \\le k \\le n} \\frac{n - k}{k}\\\\\n",
    "    &= \\sum_{1 \\le k \\le n} \\frac{n}{k} - \\sum_{1 \\le k \\le n}1\\\\\n",
    "    &= nH_n - n\n",
    "\\end{aligned}\n",
    "$$\n",
    "success!\n",
    "$$\n",
    "nH_n - n = \\sum_{0 \\le j \\lt n} H_{j}\n",
    "$$\n",
    "\n",
    "## Finite Calculus\n",
    "### Finite difference\n",
    "$$\n",
    "\\Delta f(x) = f(x + 1) - f(x)\n",
    "$$\n",
    "### Factorial Power\n",
    "#### Falling Factorial Power\n",
    "$$\n",
    "x^{\\underline{m}} = x(x - 1)...(x - m + 1) \n",
    "$$\n",
    "#### Rising Factorial Power\n",
    "$$\n",
    "x^{\\overline{m}} = x(x + 1)...(x + m - 1) \n",
    "$$\n",
    "\n",
    "### Property\n",
    "Holder for both rising and falling\n",
    "$$\n",
    "\\Delta x^{\\underline{m}} = mx^{\\underline{m - 1}}\n",
    "$$\n",
    "\n",
    "### Fundamental Thm\n",
    "$$\n",
    "g(x) = \\Delta f(x) \\iff \\sum g(x) \\delta x = f(x) + C\n",
    "$$\n",
    "\n",
    "### Bounded Finite Integral\n",
    "$$\n",
    "\\sum_a^b f(x) \\delta x = \\sum_{a \\le k \\lt b} f(k)\n",
    "$$\n",
    "\n",
    "### Useful Formula\n",
    "$$\n",
    "\\sum_{0 \\le k \\lt n}k^{\\underline{m}} =\\frac{k^{\\underline{m + 1}}}{m + 1} (\\text{from 0 to n}) = \\frac{n^{\\underline{m + 1}}}{m + 1}\n",
    "$$\n",
    "\n",
    "We can transform normal power to rasing/falling power and easily get to summation (using stirling numbers):\n",
    "$$\n",
    "k^2 = k^{\\underline{2}} + k^{\\underline 1} \\\\\n",
    "k^3 = k^{\\underline{3}} + 3k^{\\underline{2}}  + k^{\\underline 1}\n",
    "$$\n",
    "\n",
    "### Similarity to Infinite Calculus\n",
    "$$\n",
    "\\sum_{a}^bx^{\\underline{ m}}\\delta x = \\begin{cases}\n",
    "\\frac{x^{\\underline{m + 1}}}{m + 1} \\text{ from a to b}, m \\ne -1 \\\\\n",
    "H_x  \\text{ from a to b}, m = 1\n",
    "\\end{cases}\n",
    "$$\n",
    "Thus,\n",
    "$$\n",
    "\\ln x \\simeq H_x \\\\\n",
    "e^x \\simeq 2^x \n",
    "$$\n",
    "\n",
    "Define Shift Operator\n",
    "$$\n",
    "Ef(x) = f(x + 1)\n",
    "$$\n",
    "Then,\n",
    "$$\n",
    "\\Delta(uv) = u\\Delta v + Ev \\Delta u\n",
    "$$\n",
    "Integration by part:\n",
    "$$\n",
    "\\sum u \\Delta v = uv - \\sum Ev\\Delta u\n",
    "$$\n",
    "\n",
    "We can now solve $\\sum k2^k$ and $\\sum kH_k$ easily.\n",
    "\n"
   ]
  }
 ],
 "metadata": {
  "kernelspec": {
   "display_name": "Python 3",
   "language": "python",
   "name": "python3"
  },
  "language_info": {
   "codemirror_mode": {
    "name": "ipython",
    "version": 3
   },
   "file_extension": ".py",
   "mimetype": "text/x-python",
   "name": "python",
   "nbconvert_exporter": "python",
   "pygments_lexer": "ipython3",
   "version": "3.7.4"
  }
 },
 "nbformat": 4,
 "nbformat_minor": 2
}
